\input{bmsLayoutPage}
\renewcommand{\bbwAufgabenBlockID}{A1Bi}

\renewcommand{\metaHeaderLine}{Binomische Formeln}
\renewcommand{\arbeitsblattTitel}{Binomische Formeln}

\begin{document}
\arbeitsblattHeader{}

Schreiben Sie ohne Klammern:

\begin{bbwAufgabenBlock}
\item $(a+3)^2 = \LoesungsRaumLang{a^2+6a+9}$\abplz{3.2}
\item $(x-y)^2 = \LoesungsRaumLang{x^2-2xy+y^2}$\abplz{3.2}
\item $(6a+7b)^2 = \LoesungsRaumLang{36a^2+84ab+49b^2}$\abplz{3.2}
\item $(r-4)(r+4) = \LoesungsRaumLang{r^2-16}$\abplz{3.2}
\item $(3a+2b)(3a-2b) = \LoesungsRaumLang{9a^2-4b^2}$\abplz{3.2}\newpage
\item $(r^5 + s^5)^2 = \LoesungsRaumLang{r^{10} + 2r^5s^5+s^{10}}$\abplz{3.2}
\item $(c^2-1)(c^2+1) = \LoesungsRaumLang{c^4-1}$\abplz{3.2}
\item $(a-(-b))^2 = \LoesungsRaumLang{a^2+2ab+b^2}$\abplz{3.2}
\item $(-p^2-p)^2 = \LoesungsRaumLang{p^4+2p^3+p^2}$\abplz{3.2}
\item $(\frac12x+\frac13)(\frac12x-\frac13)= \LoesungsRaumLang{\frac{x^2}4 - \frac19}$\abplz{3.2}\newpage
\item $(3b+\frac16)^2 = \LoesungsRaumLang{9b^2+b+\frac1{36}}$\abplz{3.2}
\end{bbwAufgabenBlock}
\noTRAINER{\newpage}
%%\platzFuerBerechnungenBisEndeSeite{}

Verwandeln Sie in eine m√∂glichst einfache Summe:

\begin{bbwAufgabenBlock}
\item $x(x-3^2) = \LoesungsRaumLang{x^2-9x}$\abplz{4}
\item $(s+\frac12)^2\cdot{}s = \LoesungsRaumLang{s^3+s^2+\frac{s}4}$\abplz{4}
\item $(a+b+1)(a+1\cdot{}b-1) = \LoesungsRaumLang{a^2+2ab+b^2 - 1}$\abplz{4}
\item $(z^2-z-1)(z^2+z+1) = \LoesungsRaumLang{z^4-z^2-2z-1}$\abplz{4}\newpage
\item $(3-x)^2 - (x+3)(3-x)+(x+3)^2 = \LoesungsRaumLang{3x^2+9}$\abplz{4}
\item $18x + (x-9)^2 = \LoesungsRaumLang{x^2 + 81}$\abplz{4}
\item $(\sqrt{2} + \sqrt{3}b)^2 = \LoesungsRaumLang{2 +2\cdot{}\sqrt{6}\cdot{}b+3b^2}$\abplz{4}
\item $3i^2((t-i)^2-(t(s-s)-i(t+i))) = \LoesungsRaumLang{3i^2t^2 - 3ti^3 + 6i^4}$\abplz{4}\newpage
\item $(x+1)^4 = \LoesungsRaumLang{x^4+4x^3+6x^2+4x+1}$\abplz{4}
\end{bbwAufgabenBlock}
%%\platzFuerBerechnungenBisEndeSeite{}

\end{document}
