\subsection{Substitution}

Beispiel

$$\left(x+\frac1{4x} \right)^2  - 2\left(x+\frac1{4x}\right) = -1$$

\TNT{13.2}{
Ersetzte (= Substitution)$T:=\left(x+\frac1{4x}\right)$

$$T^2 - 2T = -1$$
$$T^2 - 2T + 1 = 0$$
$$(T-1)\cdot{}(T-1) = 0$$
$$T = 1$$

RÃ¼cksubstitution:

$$T = \left(x+\frac1{4x} \right)$$
mit $T=1$ wird zu
$$1 = \left( x + \frac1{4x} \right)$$
Mit $4x$ multiplizieren
$$4x = 4x^2 + 1$$
$$4x^2 -4x + 1 = 0$$
$$(2x-1)^2 = 0$$
ergo
$$\lx = \{0.5\}$$
}%% end TNT


\subsection*{Aufgaben}

\olatLinkArbeitsblatt{GlQuad}{https://olat.bms-w.ch/auth/RepositoryEntry/6029786/CourseNode/111365560138736}{Aufgabe 14. a) bis d)}
